wip

src/bounce.v
@@ -5,7 +5,7 @@ From iris.base_logic Require Import lib.ghost_var.
 
 (* This code is written in HeapLang, a simple ML-like language shipped with
 Iris. *)
-From iris.heap_lang Require Import proofmode notation adequacy.
+From iris.heap_lang Require Import proofmode notation adequacy assert.
 From iris.heap_lang.lib Require Import lock spin_lock.
 
 Require Import Bool.
@@ -13,7 +13,7 @@ Require Import Bool.
 (* set some Coq options for basic sanity *)
 (* https://coq.inria.fr/distrib/V8.13.0/refman/proofs/writing-proofs/proof-mode.html#proof-using-options
 *)
-Set Default Proof Using "Type".
+Set Default Proof Using "All".
 (* Using Default Goal Selector with the ! selector forces tactic scripts to keep
 focus to exactly one goal (e.g. using bullets) or use explicit goal selectors.*)
 Set Default Goal Selector "!".
@@ -22,7 +22,254 @@ Set Printing Projections.
 There is also something like nat_scope, probably both from Coq. *)
 Open Scope Z_scope.
 
-Definition new_bounce_unit: val :=
+
+Section bounce_code.
+
+  Definition new_bounce_unit : val :=
+    λ: "id",
+    let: "id_ref" := ref "id" in
+    let: "phase_ref" := ref #1 in
+    ("id_ref", "phase_ref").
+
+  Definition get_id : val :=
+    λ: "bounce_unit",
+    let: "id" := !(Fst "bounce_unit") in
+    "id".
+
+  Definition set_id: val :=
+    λ: "bounce_unit" "new_id",
+    let: "id_ref" := Fst "bounce_unit" in
+    "id_ref" <- "new_id";;
+    #().
+
+  Definition get_phase: val :=
+    λ: "bounce_unit",
+    let: "phase" := !(Snd "bounce_unit") in
+    "phase".
+
+  Definition phase_transit: val :=
+    λ: "bounce_unit",
+    let: "phase_ref" := !(Snd "bounce_unit") in
+    match !"phase_ref" with
+    | #1 => "phase_ref" <- #2
+    | #2 => "phase_ref" <- #3
+    | #3 => "phase_ref" <- #1
+    | _ => assert: #false (* don't handle all other cases. *)
+    end.
+
+End bounce_code.
+
+Section bounce_spec.
+Context `{!heapGS Σ, lockG Σ}.
+
+Local Notation iProp := (iProp Σ).
+
+Definition is_bounce_unit (b: val) (id: val): iProp :=
+  (∃ (id_ref phase_ref: loc), ⌜b = (#id_ref, #phase_ref)%V⌝ ∗ id_ref ↦ id)%I.
+
+
+Theorem wp_new_bounce_unit (id: val):
+  {{{ True }}}
+  new_bounce_unit id
+  {{{b, RET b; is_bounce_unit b id}}}.
+Proof.
+  iIntros (Φ) "_ HΦ".
+  wp_rec.
+  wp_alloc id_ref as "Hid".
+  wp_alloc phase_ref as "Hphase".
+  wp_pures.
+  iModIntro.
+  iApply "HΦ".
+  iExists _, _; by iFrame.
+Qed.
+
+Theorem wp_get_id (b: val) (id: val):
+  {{{ is_bounce_unit b id }}}
+    get_id b
+  {{{id, RET id; True }}}.
+Proof.
+  iIntros (Φ) "Hb HΦ".
+  iDestruct "Hb" as (id_ref phase_ref) "[% Hi]"; subst.
+  wp_rec.
+  wp_pures.
+  wp_load.
+  wp_pures.
+  iModIntro.
+  iApply "HΦ".
+  auto.
+Qed.
+
+Theorem wp_set_id (b: val) (id: val) (id': val):
+  {{{ is_bounce_unit b id }}}
+    set_id b id'
+  {{{RET #(); is_bounce_unit b id'}}}.
+  iIntros (Φ) "Hb HΦ".
+  iDestruct "Hb" as (id_ref phase_ref) "[% Hi]"; subst.
+  wp_rec.
+  wp_pures.
+  wp_store.
+  iApply "HΦ".
+  iModIntro.
+  iExists _, _; by iFrame.
+Qed.
+
+
+(*
+Theorem wp_new_bounce_unit (id: val):
+  {{{ True }}}
+    new_bounce_unit id
+  {{{b, RET b; is_bounce_unit b id}}}.
+Proof.
+  iIntros (Φ) "_ HΦ".
+  wp_rec.
+  wp_alloc id_ref as "Hid".
+  wp_alloc phase_ref as "Hphase".
+  wp_pures.
+  iModIntro.
+  iApply "HΦ".
+  iExists _, _, _.
+  iSplit.
+  - by iFrame.
+  - iFrame.
+Qed.
+
+Theorem wp_get_id (b: val) (id: val):
+  {{{ is_bounce_unit b id }}}
+    get_id b
+  {{{id, RET id; True}}}.
+Proof.
+  iIntros (Φ) "Hb HΦ".
+  wp_pures.
+  iDestruct "Hb" as (id_ref phase_ref phase) "[% [Hi Hp]]"; subst.
+  wp_rec.
+  wp_pures.
+  wp_load.
+  wp_let.
+  iModIntro.
+  iApply "HΦ".
+  auto.
+Qed.
+
+Theorem wp_set_id (b: val) (id: val) (id': val):
+  {{{ is_bounce_unit b id }}}
+    set_id b id'
+  {{{RET #(); is_bounce_unit b id'}}}.
+Proof.
+  iIntros (Φ) "Hb HΦ".
+  iDestruct "Hb" as (id_ref p_ref phase)  "[% [Hi Hp]]"; subst.
+  wp_lam.
+  wp_pures.
+  wp_store.
+  unfold is_bounce_unit.
+  iDestruct "HΦ" as (id_ref' p_ref' phase') "[Hb [Hi Hp]]".
+  iApply "HΦ".
+
+
+
+
+
+
+
+Lemma get_id_spec (b: val):
+  {{{ is_bounce_unit b }}}
+    get_id b
+  {{{ id, RET id; ⌜(id = #0)%V⌝ }}}.
+Proof.
+  iIntros (Φ) "Hb HΦ".
+  iDestruct "Hb" as
+  iDestruct
+  wp_rec.
+  wp_pures.
+
+  wp_load.
+  wp_pures.
+  iModIntro.
+  iApply "HΦ".
+  iPureIntro.
+  reflexivity.
+Qed.
+
+Lemma set_id_spec (b: val) (i: val) :
+  {{{ is_bounce_unit b}}}
+    set_id b i;;
+    get_id b
+  {{{ id, RET id; ⌜(id = i)%V⌝}}}.
+Proof.
+  iIntros (Φ) "Hb HΦ".
+  iDestruct "Hb" as (id_ref p_ref) "[% [Hi Hp]]"; subst.
+  wp_lam.
+  wp_pures.
+  wp_store.
+  wp_pures.
+  wp_lam.
+  wp_pures.
+  wp_load.
+  wp_let.
+  iModIntro.
+  iApply "HΦ".
+  iPureIntro.
+  reflexivity.
+Qed.
+
+Lemma get_phase_sepc (b: val) (i: val) (p: val):
+  {{{ is_bounce_unit b i p }}}
+    get_phase b
+  {{{ phase, RET phase; ⌜(phase = p)%V⌝ }}}.
+Proof.
+  iIntros (Φ) "Hb HΦ".
+  unfold is_bounce_unit.
+  iDestruct "Hb" as (id_ref phase_ref) "[% [Hi Hp]]"; subst.
+  wp_rec.
+  wp_pures.
+  wp_load.
+  wp_let.
+  iModIntro.
+  iApply "HΦ".
+  iPureIntro.
+  reflexivity.
+Qed.
+
+Definition phase_transit_demo: val :=
+  λ: <>,
+  let: "b" := new_bounce_unit #() in
+  Fork(phase_transit "b");;
+  let: "ok" := (get_phase "b") = #2 in
+  "ok".
+
+Theorem wp_phase_transit_demo:
+  {{{ True }}}
+  phase_transit_demo #()
+  {{{ RET #true; True}}}.
+Proof.
+  iIntros (Φ) "_ HΦ".
+  wp_rec.
+  wp_apply new_bounce_unit_spec; first auto.
+  iIntros (b) "#Hb". wp_pures.
+  wp_apply wp_fork.
+  - wp_rec.
+  wp_pure.
+  wp_let.
+  wp_rec.
+
+Lemma phase_inv (b: val) (i: val) (p: val):
+  {{{ is_bounce_unit b i p ∗  }}}
+    phase_transit b;; get_phase b
+  {{{ p', RET p'; ⌜p' = #1 ∨ p' = #2 ∨ p' = #3⌝%V  }}}.
+Proof.
+  iIntros (Φ) "Hb HΦ".
+  iDestruct "Hb" as (id_ref phase_ref) "[% [Hi Hpref]]"; subst.
+  wp_rec.
+  iCombine "Hp Hpref" as "Hp'".
+  iRewrite
+
+  wp_rec.
+  wp_pures.
+  wp_load.
+
+End bounce_spec. *)
+
+
+(* Definition new_bounce_unit: val :=
   λ: "id",
   let: "id_ref" := ref "id" in
   let: "phase" := ref #1 in
@@ -59,16 +306,16 @@ Context `{!lockG Σ}.
 Context `{!ghost_varG Σ Z}.
 Let N := nroot.@"check".
 
-Definition bounce_unit_inv (b: val) :iProp Σ :=
+Definition bounce_unit_inv (b: val) id :iProp Σ :=
   ∃ (id_ref phase_ref signed_ref num_precommits_ref num_noncommits_ref: loc),
       ⌜b = (
         #id_ref, #phase_ref, #signed_ref,
-        #num_precommits_ref, #num_noncommits_ref)%V⌝.
+        #num_precommits_ref, #num_noncommits_ref)%V⌝ ∗ id_ref ↦ id.
 
 Lemma check_new_bounce_unit:
     {{{ True }}}
         new_bounce_unit #1
-    {{{b, RET b; bounce_unit_inv b }}}.
+    {{{b, RET b; bounce_unit_inv b #1 }}}.
 Proof.
   iIntros (Φ) "_ HΦ".
   wp_rec.
@@ -81,16 +328,54 @@ Proof.
   wp_pures.
   iModIntro.
   iApply "HΦ".
-  iExists _, _, _, _, _; by iFrame.
+  iExists _, _, _, _, _.
+  iSplit.
+  { by iFrame.  }
+  by iFrame.
 Qed.
-End check.
+
+Definition get_id_inv (b:val) : iProp Σ :=
+  ∃ (id_ref: loc), ⌜get_id b = #id_ref%V⌝ ∗ ∃ (id: Z), id_ref ↦ #id.
+
+Theorem wp_get_id:
+  {{{ True }}}
+    new_bounce_unit #1
+  {{{b, RET b; get_id_inv b}}}.
+Proof.
+  iIntros (Φ) "_ HΦ".
+  unfold bounce_unit_inv.
+  wp_rec.
+  wp_alloc id_ref as "Hid".
+  wp_alloc phase_ref as "Hphase".
+  wp_alloc signed_ref as "Hsigned".
+  wp_alloc num_precommits_ref as "Hnum_precommits".
+  wp_alloc num_noncommits_ref as "Hnum_noncommits".
+
+  wp_let.
+  wp_pures.
+  iModIntro.
+  iApply "HΦ".
+  unfold get_id_inv.
+  iExists id_ref.
+  iSplit.
+  {
+    iPureIntro.
+  }
 
 
+  iPureIntro.
+  unfold get_id.
+  simpl.
+
+
+End check. *)
+
+(*
 Definition new_bounce_unit: val :=
     λ: <>,
     let: "phase" := ref #1 in
     let: "some_other" := ref #2 in
-    ("phase", "some_other").
+    ("phase", "some_other"). *)
 
 (*
     ("phase", ("second", "third"))
@@ -120,7 +405,7 @@ Definition phase_transition : val :=
     if Zeq_bool "phase" 3 then (Fst "bounce_unit") <- #1 else Fst("bounce_unit") <- "phase" + #1
     #(). *)
 
-Definition phase_transition: val :=
+(* Definition phase_transition: val :=
     λ: "bounce",
     let: "phase" := Fst "bounce" in
     match !"phase" with
@@ -146,12 +431,12 @@ Definition check_phase: val :=
 (* Define messages *)
 Inductive message: Type :=
     | Precommit
-    | Noncommit
+    | Noncommit *)
 
 
 (* This function returns a list or array of bounce units, which we call a
 flock *)
-Definition new_flock: val:=
+(* Definition new_flock: val:=
     λ: <>,
     #1.
 
@@ -197,7 +482,7 @@ Proof.
 
     (* TODO *)
 Admitted.
-End proof.
+End proof. *)
 
 (* When do you need to use Iris over Coq?
 For this just Coq would not be enough.
